cedar-dafny/pe/soundness.dfy
@@ -19,113 +19,99 @@ module pe.soundness {
   import util
   import eval
 
+  ghost predicate wellFormed(q: core.Request, s: core.EntityStore, Q: definition.Request, S: definition.EntityStore, env: Environment) {
+    env.wellFormed() && restrictedEntityStore(S) && (var pr := env.replaceUnknownInRequest(Q); pr.Some? && pr.value == q) &&
+    (var ps := env.replaceUnknownInEntityStore(S); ps.Some? && ps.value == s)
+  }
+
+  ghost predicate isSound(e: definition.Expr, q: core.Request, s: core.EntityStore, Q: definition.Request, S: definition.EntityStore, env: Environment)
+    requires env.wellFormed()
+  {
+    var peRes := PartialEvaluator(Q, S).interpret(e);
+    // If PE succeeds, then evaluating the residual and evaluating the original expression with the same unknown to value mappings should agree.
+    (peRes.Ok? ==> util.relaxedEq(ce.Evaluator(q, s).interpret(env.replaceUnknownInExpr(e)), env.interpret(peRes.value, s))) &&
+    // If PE fails, then evaluating the original expression with any uknown to value mappings should fail.
+    (peRes.Err? ==> ce.Evaluator(q, s).interpret(env.replaceUnknownInExpr(e)).Err?)
+  }
+
   lemma PEIsSoundSet(e: definition.Expr, es: seq<definition.Expr>, q: core.Request, s: core.EntityStore, Q: definition.Request, S: definition.EntityStore, env: Environment)
     requires e == definition.Expr.Set(es)
-    requires env.wellFormed() && restrictedEntityStore(S) && (var pr := env.replaceUnknownInRequest(Q); pr.Some? && pr.value == q) &&
-             (var ps := env.replaceUnknownInEntityStore(S); ps.Some? && ps.value == s)
-    ensures var peRes := PartialEvaluator(Q, S).interpret(e);
-            (peRes.Ok? ==> util.relaxedEq(ce.Evaluator(q, s).interpret(env.replaceUnknownInExpr(e)), env.interpret(peRes.value, s))) &&
-            (peRes.Err? ==> ce.Evaluator(q, s).interpret(env.replaceUnknownInExpr(e)).Err?) {
+    requires wellFormed(q, s, Q, S, env)
+    ensures isSound(e, q, s, Q, S, env) {
     var PE := PartialEvaluator(Q, S);
     var CE := ce.Evaluator(q, s);
     var peRes := PartialEvaluator(Q, S).interpret(e);
-    forall e' | e' in es {
-      PEIsSound(e', q, s, Q, S, env);
-    }
+    var ceRes := CE.interpret(env.replaceUnknownInExpr(e));
     var rs := PE.interpretSeq(es);
     eval.PEInterpretSetMapReduce(es, PE);
-    eval.CEInterpretSet(e, CE, env);
 
     var ceI := e' requires e' < e => CE.interpret(env.replaceUnknownInExpr(e'));
     var envI := e' requires PE.interpret(e').Ok? => env.interpret(PE.interpret(e').value, s);
-    assert CE.interpret(env.replaceUnknownInExpr(e)) == util.CollectToSet(util.Map(es, ceI)).Map(v => core.Value.Set(v));
+
+    assert ceRes == util.CollectToSet(util.Map(es, ceI)).Map(v => core.Value.Set(v)) by {
+      eval.CEInterpretSet(e, CE, env);
+    }
     if rs.Ok? {
       eval.PEInterpretSeqOk(es, PE);
       util.CollectToSeqOk(util.Map(es, PE.interpret));
       assert
         rs.value ==
-        util.Map(util.Map(es, PE.interpret), (r: definition.Result<Residual>) requires r.Ok? => r.value) ==
         util.Map(es, e' requires PE.interpret(e').Ok? => PE.interpret(e').value);
-
       assert forall i: nat | i < |rs.value| :: rs.value[i] == PE.interpret(es[i]).value;
 
       if (forall r | r in rs.value :: r.Concrete?) {
-        calc == {
-          env.interpret(peRes.value, s);
-          env.interpret(PE.splitSeqToSet(rs.value), s);
-          env.interpret(Concrete(core.Value.Set(set x | x in rs.value :: x.v)), s);
+        assert
+          env.interpret(peRes.value, s) ==
           Ok(core.Value.Set(set x | x in rs.value :: x.v));
-        }
-
         assert forall i: nat | i < |es| :: env.interpret(PE.interpret(es[i]).value, s).Ok?;
         assert forall e' | e' in es :: env.interpret(PE.interpret(e').value, s).Ok?;
-        assert forall e' | e' in es :: env.interpret(PE.interpret(e').value, s) == CE.interpret(env.replaceUnknownInExpr(e'));
-        util.MapEqvFunc(es, ceI, envI);
-        assert forall e' | e' in es :: e' < e && PE.interpret(e').Ok?;
-        calc == {
-          util.Map(es, ceI);
-          util.Map(es, envI);
+        assert forall e' | e' in es :: env.interpret(PE.interpret(e').value, s) == CE.interpret(env.replaceUnknownInExpr(e')) by {
+          forall e' | e' in es {
+            PEIsSound(e', q, s, Q, S, env);
+          }
         }
+        util.MapEqvFunc(es, ceI, envI);
         calc == {
           util.Map(rs.value, r => env.interpret(r, s));
           util.Map(util.Map(es, e' requires PE.interpret(e').Ok? => PE.interpret(e').value), r => env.interpret(r, s));
           util.Map(es, envI);
         }
-        assert util.Map(e.es, e' => CE.interpret(env.replaceUnknownInExpr(e'))) == util.Map(rs.value, r => env.interpret(r, s));
+        assert util.Map(es, e' => CE.interpret(env.replaceUnknownInExpr(e'))) == util.Map(rs.value, r => env.interpret(r, s));
         calc == {
           util.Map(rs.value, r => env.interpret(r, s));
           util.Map(rs.value, (r: Residual) requires r.Concrete? => Ok(r.v));
         }
         util.CollectToSetWithMap(rs.value, (r: Residual) requires r.Concrete? => definition.Result<core.Value>.Ok(r.v));
         assert util.CollectToSet(util.Map(rs.value, (r: Residual) requires r.Concrete? => definition.Result<core.Value>.Ok(r.v))).value == set x | x in rs.value :: x.v;
-        calc == {
-          CE.interpret(env.replaceUnknownInExpr(e));
-          util.CollectToSet(util.Map(e.es, envI)).Map(v => core.Value.Set(v));
-          util.CollectToSet(util.Map(rs.value, r => env.interpret(r, s))).Map(v => core.Value.Set(v));
-          util.CollectToSet(util.Map(rs.value, (r: Residual) requires r.Concrete? => Ok(r.v))).Map(v => core.Value.Set(v));
+        assert
+          CE.interpret(env.replaceUnknownInExpr(e)) ==
           Ok(core.Value.Set(set x | x in rs.value :: x.v));
-        }
       } else {
         eval.PEInterpretSet(e, PE, env, s);
-
         var rs1 := util.Map(es, envI);
         var rs2 := util.Map(es, ceI);
-        assert CE.interpret(env.replaceUnknownInExpr(e)) == util.CollectToSet(rs2).Map(v => core.Value.Set(v));
-        assert (forall i: nat | i < |es| :: PE.interpret(es[i]).Ok?) && env.interpret(PE.interpret(e).value, s) == util.CollectToSet(rs1).Map(v => core.Value.Set(v));
         assert forall i : nat | i < |es| :: util.relaxedEq(ceI(es[i]), envI(es[i])) by {
-          forall i : nat | i < |es| {
+          forall i : nat | i < |es| ensures util.relaxedEq(ceI(es[i]), envI(es[i])) {
             PEIsSound(es[i], q, s, Q, S, env);
           }
         }
-        //util.MapRel(es, ceI, envI, util.relaxedEq);
-        assert CE.interpret(env.replaceUnknownInExpr(e)) ==
-               util.CollectToSet(rs2).Map(v => core.Value.Set(v));
-        assert util.relaxedEqSeq(rs1, rs2);
         util.CollectToSetRelaxedEq(rs1, rs2);
       }
     } else {
       eval.PEInterpretSeqErr(es, PE);
-      assert exists e' | e' in es :: PE.interpret(e').Err?;
-      assert exists e' | e' in es :: CE.interpret(env.replaceUnknownInExpr(e')).Err?;
-      assert exists i: nat | i < |es| :: CE.interpret(env.replaceUnknownInExpr(es[i])).Err?;
+      var e' :| e' in es && PE.interpret(e').Err?;
+      assert ceI(e').Err? by {
+        PEIsSound(e',q, s, Q, S, env);
+      }
       util.MapExists(es, ceI, (v: definition.Result<core.Value>) => v.Err?);
-      assert exists r: definition.Result<core.Value>
-          | r in util.Map(e.es, ceI) :: r.Err?;
-      util.CollectToSetErr(util.Map(e.es, ceI));
-      assert util.CollectToSet(util.Map(e.es, ceI)).Err?;
-      assert CE.interpret(env.replaceUnknownInExpr(e)) ==
-             util.CollectToSet(util.Map(es, ceI)).Map(v => core.Value.Set(v));
-      assert CE.interpret(env.replaceUnknownInExpr(e)).Err?;
+      util.CollectToSetErr(util.Map(es, ceI));
     }
   }
 
   lemma PEIsSoundAnd(e: definition.Expr, e1: definition.Expr, e2: definition.Expr, q: core.Request, s: core.EntityStore, Q: definition.Request, S: definition.EntityStore, env: Environment)
     requires e == definition.Expr.And(e1, e2)
-    requires env.wellFormed() && restrictedEntityStore(S) && (var pr := env.replaceUnknownInRequest(Q); pr.Some? && pr.value == q) &&
-             (var ps := env.replaceUnknownInEntityStore(S); ps.Some? && ps.value == s)
-    ensures var peRes := PartialEvaluator(Q, S).interpret(e);
-            (peRes.Ok? ==> util.relaxedEq(ce.Evaluator(q, s).interpret(env.replaceUnknownInExpr(e)), env.interpret(peRes.value, s))) &&
-            (peRes.Err? ==> ce.Evaluator(q, s).interpret(env.replaceUnknownInExpr(e)).Err?)
+    requires wellFormed(q, s, Q, S, env)
+    ensures isSound(e, q, s, Q, S, env)
   {
     var PE := PartialEvaluator(Q, S);
     var CE := ce.Evaluator(q, s);
@@ -144,10 +130,42 @@ module pe.soundness {
     }
     match PE.interpret(e1) {
       case Ok(r1) => match r1 {
-        case Concrete(v1) => assume false;
+        case Concrete(v1) =>
+          assert {:focus} true;
+          match core.Value.asBool(v1) {
+            case Ok(b1) =>
+            case Err(_) =>
+          }
         case _ =>
           match PE.interpret(e2) {
-            case Ok(r2) => assume false;
+            case Ok(r2) =>
+              calc == {
+                ceRes;
+                CE.interpret(core.Expr.And(reE1, reE2));
+              }
+              assert util.relaxedEq(ceRes1, env.interpret(r1, s));
+              assert util.relaxedEq(ceRes2, env.interpret(r2, s));
+              if ceRes1.Ok? {
+                assert env.interpret(r1, s).Ok?;
+                if core.Value.asBool(env.interpret(r1, s).value).Err? {
+                  assert env.interpret(Residual.And(r1, r2), s).Err?;
+                  assert core.Value.asBool(ceRes1.value).Err?;
+                  assert  CE.interpret(core.And(reE1, reE2)).Err?;
+                } else {
+                  var b := core.Value.asBool(env.interpret(r1, s).value).value;
+                  assert ceRes1.Ok?;
+                  assert ceRes1.value == core.Value.Bool(b);
+                  if b {
+                    eval.EnvInterpretResidualTrue(env, r1, r2, s);
+                  }
+                }
+              } else {
+                eval.InterpretResidualAndErr(env, r1, r2, s);
+                assert env.interpret(Residual.And(r1, r2), s).Err?;
+                assert CE.interpret(reE1).Err? by {
+                  assert util.relaxedEq(env.interpret(r1, s), ceRes1);
+                }
+              }
             case Err(_) =>
               calc == {
                 peRes;
@@ -163,7 +181,6 @@ module pe.soundness {
                 assert CE.interpret(reE1).Err? by {
                   assert util.relaxedEq(env.interpret(r1, s), ceRes1);
                 }
-                assert CE.interpret(core.And(env.replaceUnknownInExpr(e1), env.replaceUnknownInExpr(e2))).Err?;
               } else {
                 if core.Value.asBool(env.interpret(r1, s).value).Err? {
                   assert env.interpret(Residual.And(r1, errV), s).Err?;
@@ -171,18 +188,15 @@ module pe.soundness {
                   assert  CE.interpret(core.And(reE1, reE2)).Err?;
                 } else {
                   var b := core.Value.asBool(env.interpret(r1, s).value).value;
-                  assert CE.interpret(env.replaceUnknownInExpr(e1)).Ok?;
-                  assert CE.interpret(env.replaceUnknownInExpr(e1)).value == core.Value.Bool(b);
+                  assert ceRes1.Ok?;
+                  assert ceRes1.value == core.Value.Bool(b);
                   if b {
                     eval.MakeErrorValueIsErr(env, s);
-                    assert CE.interpret(env.replaceUnknownInExpr(e2)).Err?;
+                    assert ceRes2.Err?;
                     assert CE.interpret(core.And(env.replaceUnknownInExpr(e1), env.replaceUnknownInExpr(e2))) == CE.interpret(env.replaceUnknownInExpr(e2));
                     assert CE.interpret(env.replaceUnknownInExpr(e)).Err?;
                     assert env.interpret(Residual.And(r1, PE.makeErrorValue()), s) == env.interpret(PE.makeErrorValue(), s);
                     assert env.interpret(PE.makeErrorValue(), s).Err?;
-                  } else {
-                    assert CE.interpret(core.And(env.replaceUnknownInExpr(e1), env.replaceUnknownInExpr(e2))) == Ok(core.Value.Bool(false));
-                    assert  env.interpret(Residual.And(r1, PE.makeErrorValue()), s) == Ok(core.Value.Bool(false));
                   }
                 }
               }
@@ -195,13 +209,8 @@ module pe.soundness {
 
   lemma PEIsSound(e: definition.Expr, q: core.Request, s: core.EntityStore, Q: definition.Request, S: definition.EntityStore, env: Environment)
     decreases e
-    requires env.wellFormed() && restrictedEntityStore(S) && (var pr := env.replaceUnknownInRequest(Q); pr.Some? && pr.value == q) &&
-             (var ps := env.replaceUnknownInEntityStore(S); ps.Some? && ps.value == s)
-    ensures var peRes := PartialEvaluator(Q, S).interpret(e);
-            // If PE succeeds, then evaluating the residual and evaluating the original expression with the same unknown to value mappings should agree.
-            (peRes.Ok? ==> util.relaxedEq(ce.Evaluator(q, s).interpret(env.replaceUnknownInExpr(e)), env.interpret(peRes.value, s))) &&
-            // If PE fails, then evaluating the original expression with any uknown to value mappings should fail.
-            (peRes.Err? ==> ce.Evaluator(q, s).interpret(env.replaceUnknownInExpr(e)).Err?)
+    requires wellFormed(q, s, Q, S, env)
+    ensures isSound(e, q, s, Q, S, env)
   {
     var peRes := PartialEvaluator(Q, S).interpret(e);
     var PE := PartialEvaluator(Q, S);
@@ -233,6 +242,7 @@ module pe.soundness {
         PEIsSound(arg2, q, s, Q, S, env);
       case GetAttr(se, a) =>
         assert {:split_here} true;
+        reveal restrictedEntityStore();
         var peRes' := PartialEvaluator(Q, S).interpret(se);
         PEIsSound(se, q, s, Q, S, env);
         if peRes'.Ok? {
